coq/proof/SoundForgetMemory.v
@@ -34,77 +34,336 @@ Definition noalias_with_def_memory (conf:Config) (def_memory:option (GenericValu
          (DEF: def_memory = Some (gptr_def, ty_def)),
     InvState.Unary.sem_noalias conf gptr_def ptr ty_def ty.
 
-Inductive state_equiv_except_mem (conf:Config) (def_mptr:option (GenericValue * typ)) (st0 st1:State): Prop :=
+Inductive mem_change : Type :=
+| mem_change_alloc
+    (gsz:sz) (gn:GenericValue) (a:align)
+| mem_change_store
+    (ptr:GenericValue) (ty:typ) (gv:GenericValue) (a:align)
+| mem_change_free
+    (ptr:GenericValue)
+| mem_change_none
+.
+
+(* Definition ptr_to_genericvalue conf st invst ptr: option (GenericValue * typ) := *)
+(*   match InvState.Unary.sem_valueT conf st invst ptr.(fst) with *)
+(*   | Some gv => Some (gv, ptr.(snd)) *)
+(*   | None => None *)
+(*   end. *)
+
+Inductive mem_change_inject mi: mem_change -> mem_change -> Prop :=
+| mem_change_inject_alloc_alloc
+    gsz gn a
+  : mem_change_inject mi (mem_change_alloc gsz gn a) (mem_change_alloc gsz gn a)
+| mem_change_inject_alloc_none
+    gsz gn a
+  : mem_change_inject mi (mem_change_alloc gsz gn a) mem_change_none
+| mem_change_inject_none_alloc
+    gsz gn a
+  : mem_change_inject mi mem_change_none (mem_change_alloc gsz gn a)
+| mem_change_inject_store
+    ptr0 ptr1 gv0 gv1 ty a
+    (PTR_INJECT: genericvalues_inject.gv_inject mi ptr0 ptr1)
+    (VAL_INJECT: genericvalues_inject.gv_inject mi gv0 gv1)
+  : mem_change_inject mi (mem_change_store ptr0 ty gv0 a) (mem_change_store ptr1 ty gv1 a)
+| mem_change_inject_free
+    ptr0 ptr1
+    (PTR_INJECT: genericvalues_inject.gv_inject mi ptr0 ptr1)
+    : mem_change_inject mi (mem_change_free ptr0) (mem_change_free ptr1)
+| mem_change_inject_none
+    : mem_change_inject mi mem_change_none mem_change_none
+.
+
+Inductive mem_change_location conf st invst: mem_change -> option Ptr.t -> Prop :=
+| mem_change_location_alloc
+    bsz gn a
+  : mem_change_location conf st invst (mem_change_alloc bsz gn a) None
+| mem_change_location_store
+    ptr gv_ptr gv a
+    (STORE_PTR: InvState.Unary.sem_valueT conf st invst ptr.(fst) = Some gv_ptr)
+  : mem_change_location conf st invst (mem_change_store gv_ptr ptr.(snd) gv a) (Some ptr)
+| mem_change_location_free
+    ptr gv_ptr
+    (FREE_PTR: InvState.Unary.sem_valueT conf st invst ptr.(fst) = Some gv_ptr)
+  : mem_change_location conf st invst (mem_change_free gv_ptr) (Some ptr)
+| mem_change_location_none
+  : mem_change_location conf st invst mem_change_none None
+.
+
+Inductive mem_change_equiv (conf:Config) (mem0 mem1:mem): mem_change -> Prop :=
+| mem_change_equiv_alloc
+    mb bsz gn a
+    (MALLOC: Some (mem1, mb) = malloc conf.(CurTargetData) mem0 bsz gn a)
+  : mem_change_equiv conf mem0 mem1 (mem_change_alloc bsz gn a)
+| mem_change_equiv_store
+    ptr ty gv a
+    (STORE: Some mem1 = mstore conf.(CurTargetData) mem0 ptr ty gv a)
+  : mem_change_equiv conf mem0 mem1 (mem_change_store ptr ty gv a)
+| mem_change_equiv_free
+    ptr
+    (FREE: Some mem1 = free conf.(CurTargetData) mem0 ptr)
+  : mem_change_equiv conf mem0 mem1 (mem_change_free ptr)
+| mem_change_equiv_none
+    (MEM: mem0 = mem1)
+  : mem_change_equiv conf mem0 mem1 mem_change_none
+.
+
+Inductive state_equiv_except_mem (conf:Config) (st0 st1:State) (mem_chng:mem_change) :=
 | state_equiv_except_mem_intro
-    (LOCALS: st0.(EC).(Locals) = st1.(EC).(Locals))
-    (MEM: forall ptr ty a gv
-                 (NOALIAS: noalias_with_def_memory conf def_mptr ptr ty)
-                 (LOAD: mload conf.(CurTargetData) st0.(Mem) ptr ty a = Some gv),
-        mload conf.(CurTargetData) st1.(Mem) ptr ty a = Some gv)
+    (LOCALS_EQ: st0.(EC).(Locals) = st1.(EC).(Locals))
+    (MEM_CHANGE_EQUIV: mem_change_equiv conf st0.(Mem) st1.(Mem) mem_chng)
 .
 
 Definition unique_preserved_mem conf st inv: Prop :=
   forall u (MEM: AtomSetImpl.mem u inv.(Invariant.unique) = true),
     InvState.Unary.sem_unique conf st u.
 
-Definition ptr_to_genericvalue conf st invst ptr: option (GenericValue * typ) :=
-  match InvState.Unary.sem_valueT conf st invst ptr.(fst) with
-  | Some gv => Some (gv, ptr.(snd))
-  | None => None
-  end.
+(* Definition ptr_to_genericvalue conf st invst ptr: option (GenericValue * typ) := *)
+(*   match InvState.Unary.sem_valueT conf st invst ptr.(fst) with *)
+(*   | Some gv => Some (gv, ptr.(snd)) *)
+(*   | None => None *)
+(*   end. *)
 
-Lemma forget_memory_unary_sound
+Lemma forget_memory_unary_sound1
       conf st0 invst0 invmem0 inv0
-      def_memory st1 public
+      def_memory st1 public gmax mem_change
         (STATE: InvState.Unary.sem conf st0 invst0 invmem0 inv0)
-        (MEM_EQUIV: state_equiv_except_mem conf
-                    (ptr_to_genericvalue conf st0 invst0 def_memory) st0
-                    st1)
+        (MEM: InvMem.Unary.sem conf gmax public st0.(Mem) invmem0)
+        (MEM_EQUIV: state_equiv_except_mem conf st0 st1 mem_change)
+        (MEM_CHANGE: mem_change_location conf st0 invst0 mem_change (Some def_memory))
         (UNIQUE_PRSV: unique_preserved_mem conf st1 inv0)
-    : exists invmem1,
-      <<STATE_UNARY: InvState.Unary.sem conf st1 invst0 invmem1 (ForgetMemory.unary def_memory inv0)>> /\
-      <<MEM_UNARY: InvMem.Unary.sem conf public st1.(Mem) invmem1>> /\
-      <<MEMLE_UNARY: InvMem.Unary.le invmem0 invmem1>>.
+    : <<STATE_UNARY: InvState.Unary.sem conf st1 invst0 invmem0 (ForgetMemory.unary def_memory inv0)>> /\
+      <<MEM_UNARY: InvMem.Unary.sem conf gmax public st1.(Mem) invmem0>>.
 Proof.
 Admitted.
 
+Lemma forget_memory_unary_sound2
+      conf st0 st1 mem_change
+      invst0 invmem0 inv0 gmax public
+      (MEM: InvMem.Unary.sem conf gmax public st0.(Mem) invmem0)
+      (MEM_EQUIV : state_equiv_except_mem conf st0 st1 mem_change)
+      (MEM_CHANGE : mem_change_location conf st0 invst0 mem_change None)
+      (TGT : InvState.Unary.sem conf st0 invst0 invmem0 inv0)
+  : <<STATE_UNARY: InvState.Unary.sem conf st1 invst0 invmem0 inv0>> /\
+    <<MEM_UNARY: InvMem.Unary.sem conf gmax public st1.(Mem) invmem0>>.
+Proof.
+Admitted.
+
+Lemma some_injective A (a b:A):
+  Some a = Some b -> a = b.
+Proof.
+  congruence.
+Qed.
+
+Lemma mem_inject_change
+      conf_src mem0_src mem1_src mem_change_src
+      conf_tgt mem0_tgt mem1_tgt mem_change_tgt
+      mi
+      (MEM_CHANGE_EQUIV_SRC : mem_change_equiv conf_src mem0_src mem1_src mem_change_src)
+      (MEM_CHANGE_EQUIV_TGT : mem_change_equiv conf_tgt mem0_tgt mem1_tgt mem_change_tgt)
+      (MEM_CHANGE_INJECT : mem_change_inject mi mem_change_src mem_change_tgt)
+      (INJECT : Memory.Mem.inject mi mem0_src mem0_tgt)
+  : Memory.Mem.inject mi mem1_src mem1_tgt.
+Proof.
+  inv MEM_CHANGE_INJECT.
+  - inv INJECT. inv MEM_CHANGE_EQUIV_SRC. inv MEM_CHANGE_EQUIV_TGT.
+    unfold malloc in *.
+    apply some_injective in MALLOC.
+    apply some_injective in MALLOC0.
+    econs.
+    + eapply Memory.Mem.alloc_right_inj; eauto.
+      eapply Memory.Mem.alloc_left_unmapped_inj; eauto.
+      apply mi_freeblocks.
+      eapply Memory.Mem.fresh_block_alloc; eauto.
+    + i. apply mi_freeblocks. ii.
+      exploit Memory.Mem.valid_block_alloc; try (symmetry; exact MALLOC); eauto.
+    + ii. exploit mi_mappedblocks; eauto. i.
+      eapply Memory.Mem.valid_block_alloc; eauto.
+    + ii. exploit mi_no_overlap; eauto.
+      * eapply Memory.Mem.perm_alloc_4; try (symmetry; exact MALLOC); eauto.
+        ii. subst.
+        hexploit Memory.Mem.fresh_block_alloc; try (symmetry; exact MALLOC); eauto. i.
+        exploit mi_freeblocks; eauto. i. clarify.
+      * eapply Memory.Mem.perm_alloc_4; try (symmetry; exact MALLOC); eauto.
+        ii. subst.
+        hexploit Memory.Mem.fresh_block_alloc; try (symmetry; exact MALLOC); eauto. i.
+        exploit mi_freeblocks; eauto. i. clarify.
+    + ii. exploit mi_representable; eauto. des.
+      * left.
+        eapply Memory.Mem.perm_alloc_4; try (symmetry; exact MALLOC); eauto.
+        ii. subst.
+        hexploit Memory.Mem.fresh_block_alloc; try (symmetry; exact MALLOC); eauto. i.
+        exploit mi_freeblocks; eauto. i. clarify.
+      * right.
+        eapply Memory.Mem.perm_alloc_4; try (symmetry; exact MALLOC); eauto.
+        ii. subst.
+        hexploit Memory.Mem.fresh_block_alloc; try (symmetry; exact MALLOC); eauto. i.
+        exploit mi_freeblocks; eauto. i. clarify.
+  - inv INJECT. inv MEM_CHANGE_EQUIV_SRC. inv MEM_CHANGE_EQUIV_TGT.
+    unfold malloc in *.
+    apply some_injective in MALLOC.
+    econs.
+    + eapply Memory.Mem.alloc_left_unmapped_inj; eauto.
+      apply mi_freeblocks.
+      eapply Memory.Mem.fresh_block_alloc; eauto.
+    + i. apply mi_freeblocks. ii.
+      exploit Memory.Mem.valid_block_alloc; try (symmetry; exact MALLOC); eauto.
+    + ii. exploit mi_mappedblocks; eauto.
+    + ii. exploit mi_no_overlap; eauto.
+      * eapply Memory.Mem.perm_alloc_4; try (symmetry; exact MALLOC); eauto.
+        ii. subst.
+        hexploit Memory.Mem.fresh_block_alloc; try (symmetry; exact MALLOC); eauto. i.
+        exploit mi_freeblocks; eauto. i. clarify.
+      * eapply Memory.Mem.perm_alloc_4; try (symmetry; exact MALLOC); eauto.
+        ii. subst.
+        hexploit Memory.Mem.fresh_block_alloc; try (symmetry; exact MALLOC); eauto. i.
+        exploit mi_freeblocks; eauto. i. clarify.
+    + ii. exploit mi_representable; eauto. des.
+      * left.
+        eapply Memory.Mem.perm_alloc_4; try (symmetry; exact MALLOC); eauto.
+        ii. subst.
+        hexploit Memory.Mem.fresh_block_alloc; try (symmetry; exact MALLOC); eauto. i.
+        exploit mi_freeblocks; eauto. i. clarify.
+      * right.
+        eapply Memory.Mem.perm_alloc_4; try (symmetry; exact MALLOC); eauto.
+        ii. subst.
+        hexploit Memory.Mem.fresh_block_alloc; try (symmetry; exact MALLOC); eauto. i.
+        exploit mi_freeblocks; eauto. i. clarify.
+  - inv INJECT. inv MEM_CHANGE_EQUIV_SRC. inv MEM_CHANGE_EQUIV_TGT.
+    unfold malloc in *.
+    apply some_injective in MALLOC.
+    econs.
+    + eapply Memory.Mem.alloc_right_inj; eauto.
+    + i. apply mi_freeblocks. eauto.
+    + ii. exploit mi_mappedblocks; eauto. i.
+      eapply Memory.Mem.valid_block_alloc; eauto.
+    + ii. exploit mi_no_overlap; eauto.
+    + ii. exploit mi_representable; eauto.
+  - inv MEM_CHANGE_EQUIV_SRC. inv MEM_CHANGE_EQUIV_TGT.
+    unfold mstore in *. des_ifs.
+    (* exploit genericvalues_inject.mem_inj_mstore_aux; eauto. *)
+    
+    (* Memory.Mem.mem_inj *)
+    (*   memory_sim.MoreMem.mem_inj *)
+    admit. (* store - store *)
+  - inv MEM_CHANGE_EQUIV_SRC. inv MEM_CHANGE_EQUIV_TGT.
+    unfold free in *. des_ifs.
+    eapply Memory.Mem.free_left_inject; eauto.
+    eapply Memory.Mem.free_right_inject; eauto.
+    admit. (* free - free *)
+  - inv MEM_CHANGE_EQUIV_SRC. inv MEM_CHANGE_EQUIV_TGT.
+    econs; eauto.
+Admitted.
+
 Lemma forget_memory_sound
-      conf_src st0_src st1_src def_memory_src
-      conf_tgt st0_tgt st1_tgt def_memory_tgt
+      conf_src st0_src st1_src def_memory_src mem_change_src
+      conf_tgt st0_tgt st1_tgt def_memory_tgt mem_change_tgt
       invst0 invmem0 inv0
       (STATE: InvState.Rel.sem conf_src conf_tgt st0_src st0_tgt invst0 invmem0 inv0)
       (MEM: InvMem.Rel.sem conf_src conf_tgt st0_src.(Mem) st0_tgt.(Mem) invmem0)
       (MEM_EQUIV_SRC: state_equiv_except_mem
-                  conf_src
-                  (monad.mbind _ _ (ptr_to_genericvalue conf_src st0_src invst0.(InvState.Rel.src)) def_memory_src)
-                  st0_src st1_src)
+                        conf_src
+                        st0_src st1_src
+                        mem_change_src)
       (MEM_EQUIV_TGT: state_equiv_except_mem
-                  conf_tgt
-                  (monad.mbind _ _ (ptr_to_genericvalue conf_tgt st0_tgt invst0.(InvState.Rel.tgt)) def_memory_tgt)
-                  st0_tgt st1_tgt)
+                        conf_tgt
+                        st0_tgt st1_tgt
+                        mem_change_tgt)
+      (MEM_CHANGE_SRC: mem_change_location conf_src st0_src invst0.(InvState.Rel.src) mem_change_src def_memory_src)
+      (MEM_CHANGE_TGT: mem_change_location conf_tgt st0_tgt invst0.(InvState.Rel.tgt) mem_change_tgt def_memory_tgt)
+      (MEM_CHANGE_INJECT: mem_change_inject invmem0.(InvMem.Rel.inject) mem_change_src mem_change_tgt)
       (UNIQUE_PRSV_SRC: unique_preserved_mem conf_src st1_src inv0.(Invariant.src))
       (UNIQUE_PRSV_TGT: unique_preserved_mem conf_tgt st1_tgt inv0.(Invariant.tgt))
-  : exists invmem1,
-    <<STATE: InvState.Rel.sem conf_src conf_tgt st1_src st1_tgt invst0 invmem1
+  : <<STATE: InvState.Rel.sem conf_src conf_tgt st1_src st1_tgt invst0 invmem0
                               (ForgetMemory.t def_memory_src def_memory_tgt inv0) >> /\
-    <<MEM: InvMem.Rel.sem conf_src conf_tgt st1_src.(Mem) st1_tgt.(Mem) invmem1>> /\
-    <<MEMLE: InvMem.Rel.le invmem0 invmem1>>.
+    <<MEM: InvMem.Rel.sem conf_src conf_tgt st1_src.(Mem) st1_tgt.(Mem) invmem0>>.
 Proof.
   inv STATE.
   unfold ForgetMemory.t.
   destruct def_memory_src as [[]|], def_memory_tgt as [[]|]; ss.
-  - exploit forget_memory_unary_sound; try exact SRC; eauto. i. des.
-    exploit forget_memory_unary_sound; try exact TGT; eauto. i. des.
-    eexists (InvMem.Rel.mk _ _ _). splits; swap 2 3.
+  inv MEM.
+
+  - exploit forget_memory_unary_sound1; try exact SRC; eauto. i. des.
+    exploit forget_memory_unary_sound1; try exact TGT; eauto. i. des.
+    splits.
     + econs; ss; eauto. i.
       hexploit MAYDIFF; eauto. i.
-      admit. (* easy; use H *)
+      ii. exploit H.
+      { destruct id0 as [[]]; eauto.
+        inv MEM_EQUIV_SRC; solve_sem_idT.
+        rewrite -> LOCALS_EQ; eauto.
+      }
+      i. des.
+      esplits; eauto.
+      destruct id0 as [[]]; eauto.
+      inv MEM_EQUIV_TGT;
+        solve_sem_idT; rewrite <- LOCALS_EQ; eauto.
     + econs; ss; eauto.
+      inv MEM_EQUIV_SRC.
+      inv MEM_EQUIV_TGT.
+
+      eapply mem_inject_change; eauto.
+      
+  - inv MEM.
+    exploit forget_memory_unary_sound1; try exact SRC; eauto. i. des.
+    exploit forget_memory_unary_sound2; try exact TGT; eauto. i. des.
+    splits.
     + econs; ss; eauto.
-      inv MEM.
-      admit. (* hard; use INJECT *)
-      (* state_equiv_except_mem st0 st1 (Some (ptr, ty, a, v)) -> *)
-  - admit.
-  - admit.
-  - admit.
+      i.
+      hexploit MAYDIFF; eauto. i.
+      ii. exploit H.
+      { destruct id0 as [[]]; eauto.
+        inv MEM_EQUIV_SRC; solve_sem_idT.
+        rewrite -> LOCALS_EQ; eauto.
+      }
+      i. des.
+      esplits; eauto.
+      destruct id0 as [[]]; eauto.
+      inv MEM_EQUIV_TGT;
+        solve_sem_idT; rewrite <- LOCALS_EQ; eauto.
+    + econs; ss; eauto.
+      inv MEM_EQUIV_SRC.
+      inv MEM_EQUIV_TGT.
+      eapply mem_inject_change; eauto.
+  - inv MEM.
+    exploit forget_memory_unary_sound2; try exact SRC; eauto. i. des.
+    exploit forget_memory_unary_sound1; try exact TGT; eauto. i. des.
+    splits.
+    + econs; ss; eauto.
+      i.
+      hexploit MAYDIFF; eauto. i.
+      ii. exploit H.
+      { destruct id0 as [[]]; eauto.
+        inv MEM_EQUIV_SRC; solve_sem_idT.
+        rewrite -> LOCALS_EQ; eauto.
+      }
+      i. des.
+      esplits; eauto.
+      destruct id0 as [[]]; eauto.
+      inv MEM_EQUIV_TGT;
+        solve_sem_idT; rewrite <- LOCALS_EQ; eauto.
+    + econs; ss; eauto.
+      inv MEM_EQUIV_SRC.
+      inv MEM_EQUIV_TGT.
+      eapply mem_inject_change; eauto.
+  - inv MEM.
+    exploit forget_memory_unary_sound2; try exact SRC; eauto. i. des.
+    exploit forget_memory_unary_sound2; try exact TGT; eauto. i. des.
+    splits.
+    + econs; ss; eauto.
+      i.
+      hexploit MAYDIFF; eauto. i.
+      ii. exploit H.
+      { destruct id0 as [[]]; eauto.
+        inv MEM_EQUIV_SRC; solve_sem_idT.
+        rewrite -> LOCALS_EQ; eauto.
+      }
+      i. des.
+      esplits; eauto.
+      destruct id0 as [[]]; eauto.
+      inv MEM_EQUIV_TGT;
+        solve_sem_idT; rewrite <- LOCALS_EQ; eauto.
+    + econs; ss; eauto.
+      inv MEM_EQUIV_SRC.
+      inv MEM_EQUIV_TGT.
+      eapply mem_inject_change; eauto.
 Admitted.
